Lots of work saved, up to cvm semantics

src/Cvm_Monad.v
@@ -5,7 +5,7 @@
   Author:  Adam Petz, ampetz@ku.edu
 *)
 
-Require Import ResultT Term EvidenceT_Bundlers Axioms_Io Maps Session_Config_Compiler.
+Require Import ResultT Term Evidence_Bundlers Maps Session_Config_Compiler.
 
 Require Import Coq.Program.Tactics.
 
@@ -14,7 +14,7 @@ Require Import Manifest_Admits ErrorStringConstants Attestation_Session.
 Require Import String List.
 Import ListNotations.
 
-Require Export Cvm_St ErrorStMonad_Coq IO_Stubs Interface.
+Require Export Cvm_St ErrorStMonad_Coq IO_Stubs Interface JSON_Core Axioms_Io.
 
 Import ErrNotation.
 
@@ -69,10 +69,6 @@ Definition inc_id : CVM Event_ID :=
   err_put (mk_st e tr (Nat.add i (S O)) sc) ;;
   err_ret i.
 
-Definition modify_evm (f:Evidence -> Evidence) : CVM unit :=
-  e <- get_ev ;;
-  put_ev (f e).
-
 (* Definition add_trace (tr':list Ev) : cvm_st -> cvm_st :=
   tr <- get_trace ;;
   
@@ -101,27 +97,40 @@ Definition tag_ASP (params :ASP_PARAMS) (mpl:Plc) (e:Evidence) : CVM Event_ID :=
   add_trace [umeas x mpl params (get_et e)] ;;
   err_ret x.
 
+Definition join_seq (e1:Evidence) (e2:Evidence): CVM unit :=
+  p <- get_pl ;;
+  n <- inc_id ;;
+  put_ev (ss_cons e1 e2) ;;
+  add_trace [join n p].
+
 (* Helper function that builds a new internal EvidenceT bundle based on 
    the EvidenceT extension parameter of an ASP term. *)
-Definition fwd_asp (fwd:FWD) (rwev : RawEv) (e:Evidence) (p:Plc) (ps:ASP_PARAMS): CVM Evidence :=
-  match fwd with
-  | COMP => 
-      match comp_bundle rwev e p ps with
-      | resultC e' => err_ret e'
-      | errC e => err_failm (dispatch_error (Runtime e))
-      end
-  | EXTD n => 
-      match extd_bundle rwev e p n ps with
-      | resultC e' => err_ret e'
-      | errC e => err_failm (dispatch_error (Runtime e))
-      end
-  | ENCR => 
-      match encr_bundle rwev e p ps with
-      | resultC e' => err_ret e'
-      | errC e => err_failm (dispatch_error (Runtime e))
-      end
-  | KILL => err_ret mt_evc
-  | KEEP => err_ret e
+Definition bundle_asp (p:Plc) (rwev : RawEv) (e:Evidence) 
+    (ps:ASP_PARAMS) : CVM Evidence :=
+  sc <- get_config ;;
+  let '(asp_paramsC asp_id args targ_plc targ) := ps in
+  match (map_get (asp_types (session_context sc)) asp_id) with
+  | None => err_failm (dispatch_error (Runtime err_str_asp_no_type_sig))
+  | Some fwd =>
+    match fwd with
+    | COMP => 
+        match comp_bundle rwev e p ps with
+        | resultC e' => err_ret e'
+        | errC e => err_failm (dispatch_error (Runtime e))
+        end
+    | EXTD n => 
+        match extd_bundle rwev e p n ps with
+        | resultC e' => err_ret e'
+        | errC e => err_failm (dispatch_error (Runtime e))
+        end
+    | ENCR => 
+        match encr_bundle rwev e p ps with
+        | resultC e' => err_ret e'
+        | errC e => err_failm (dispatch_error (Runtime e))
+        end
+    | KILL => err_ret mt_evc
+    | KEEP => err_ret e
+    end
   end.
 
 (** * Stub for invoking external ASP procedures.  
@@ -136,14 +145,84 @@ Definition do_asp (params :ASP_PARAMS) (e:RawEv) (x:Event_ID) : CVM RawEv :=
 
 (* Simulates invoking an arbitrary ASP.  Tags the event, builds and returns 
    the new EvidenceT bundle. *)
-Definition invoke_ASP (fwd:FWD) (params:ASP_PARAMS) (* (ac : AM_Config) *) : CVM Evidence :=
-  e <- get_ev ;;
+Definition invoke_ASP (sp : SP) (params:ASP_PARAMS) : CVM Evidence :=
+  e <-  match sp with
+        | ALL => get_ev
+        | NONE => err_ret mt_evc
+        end ;;
   p <- get_pl ;;
   x <- tag_ASP params p e ;;
   rawev <- do_asp params (get_bits e) x ;;
-  outev <- fwd_asp fwd rawev e p params ;;
+  outev <- bundle_asp p rawev e params ;;
   err_ret outev.
 
+Fixpoint peel_n_rawev (n : nat) (ls : RawEv) : CVM (RawEv * RawEv) :=
+  match n with
+  | 0 => err_ret ([], ls)
+  | S n' =>
+    match ls with
+    | [] => err_failm (dispatch_error (Runtime errStr_peel_n_am))
+    | x :: ls' =>
+      v <- peel_n_rawev n' ls' ;;
+      match v with
+      | (ls1, ls2) => err_ret (x :: ls1, ls2)
+      end
+    end
+  end.
+
+Definition split_evidence (r : RawEv) (et1 et2 : EvidenceT) 
+    : CVM (Evidence * Evidence) :=
+  sc <- get_config ;;
+  let G := (session_context sc) in
+  match et_size G et1 with
+  | errC e => err_failm (dispatch_error (Runtime e))
+  | resultC et1_size => 
+    match et_size G et2 with
+    | errC e => err_failm (dispatch_error (Runtime e))
+    | resultC et2_size =>
+      '(l_ev, rest) <- peel_n_rawev et1_size r ;;
+      '(r_ev, rest') <- peel_n_rawev et2_size rest ;;
+      match rest' with
+      | [] => err_ret (evc l_ev et1, evc r_ev et2)
+      | _ => err_failm (dispatch_error (Runtime "Evidence splitting failed!"))
+      end
+    end
+  end.
+
+(* Simulates invoking an arbitrary ASP.  Tags the event, builds and returns 
+   the new EvidenceT bundle. *)
+
+Fixpoint invoke_APPR (et : EvidenceT) : CVM unit :=
+  match et with
+  | mt_evt => put_ev mt_evc (* appraise nothing = mt *)
+  | nonce_evt n' => 
+      ev' <- invoke_ASP ALL check_nonce_params ;;
+      put_ev ev'
+  | asp_evt p' par et' =>
+    sc <- get_config ;;
+    let '(asp_paramsC asp_id args targ_plc targ) := par in
+    match (map_get (asp_comps (session_context sc)) asp_id) with
+    | None => err_failm (dispatch_error (Runtime err_str_asp_no_compat_appr_asp))
+    | Some appr_asp_id =>
+      ev' <- invoke_ASP ALL (asp_paramsC appr_asp_id args targ_plc targ) ;;
+      put_ev ev'
+    end
+  | split_evt et1 et2 =>
+    split_ev ;; (* register event that we are splitting evidence *)
+    (* first we must get out the actual Evidence for et1 *)
+    top_ev <- get_ev ;;
+    '(e1, e2) <- split_evidence (get_bits top_ev) et1 et2 ;;
+    (* put ev for e1 to act on *)
+    put_ev e1 ;;
+    invoke_APPR et1 ;;
+    ev1' <- get_ev ;;
+    (* put ev for e2 to act on *)
+    put_ev e2 ;;
+    invoke_APPR et2 ;;
+    ev2' <- get_ev ;;
+    join_seq ev1' ev2' 
+  end.
+    
 Definition copyEv : CVM Evidence :=
   p <- get_pl ;;
   x <- inc_id ;;
@@ -160,14 +239,19 @@ Definition clearEv : unit -> CVM Evidence :=
   fun _ => err_ret mt_evc.
 
 (* Helper that interprets primitive core terms in the CVM.  *)
-Definition do_prim (a:ASP_Core) (* (ac : AM_Config) *) : CVM Evidence :=
+Definition do_prim (a: ASP) : CVM Evidence :=
   match a with
-  | NULLC => nullEv
-  | CLEAR => clearEv tt
-  | CPYC => copyEv
-  | ASPCC fwd params => invoke_ASP fwd params
+  | NULL => nullEv
+  | CPY => copyEv
+  | ASPC sp params => invoke_ASP sp params
+  | SIG => invoke_ASP ALL sig_params
+  | HSH => invoke_ASP ALL hsh_params
+  | APPR => 
+    e <- get_ev ;;
+    invoke_APPR (get_et e) ;;
+    get_ev
+  | ENC q => invoke_ASP ALL (enc_params q)
   end.
-
 
 (* event_id_span functions were HERE *)
 
@@ -176,13 +260,25 @@ Definition do_prim (a:ASP_Core) (* (ac : AM_Config) *) : CVM Evidence :=
    corresponding to the size of a Term *)
 Definition inc_remote_event_ids (t:Term) : CVM unit :=
   i <- get_evid ;;
-  put_evid (Nat.add i (event_id_span' t)).
+  sc <- get_config ;;
+  p <- get_pl ;;
+  ev <- get_ev ;;
+  match (events_size (session_context sc) p (get_et ev) t) with
+  | errC e => err_failm (dispatch_error (Runtime e))
+  | resultC n => put_evid (Nat.add i n)
+  end.
 
 (* Monadic helper function to simulate a span of parallel event IDs 
-   corresponding to the size of a Core_Term *)
-Definition inc_par_event_ids (t:Core_Term) : CVM unit :=
+   corresponding to the size of a Term *)
+Definition inc_par_event_ids (t: Term) : CVM unit :=
   i <- get_evid ;;
-  put_evid (Nat.add i (event_id_span t)).
+  sc <- get_config ;;
+  p <- get_pl ;;
+  ev <- get_ev ;;
+  match (events_size (session_context sc) p (get_et ev) t) with
+  | errC e => err_failm (dispatch_error (Runtime e))
+  | resultC n => put_evid (Nat.add i n)
+  end.
   
 (* Primitive monadic communication primitives 
    (some rely on Admitted IO Stubs). *)
@@ -208,8 +304,10 @@ Definition check_cvm_policy (t:Term) (pTo:Plc) (et:EvidenceT) : CVM unit :=
     | true => err_ret tt
     | false => err_failm (dispatch_error (Runtime errStr_disclosePolicy))
     end.
+    
+(* Remote communication primitives *)
 
-Definition do_remote (t:Term) (pTo:Plc) (e:Evidence) (sc : Session_Config) 
+Definition do_remote (sc : Session_Config) (pTo: Plc) (e : Evidence) (t:Term) 
     : ResultT RawEv DispatcherErrors := 
   (* There is assuredly a better way to do it than this *)
   let '(mkAtt_Sesplit_evt my_plc plc_map pk_map) := (session_config_decompiler sc) in
@@ -219,7 +317,7 @@ Definition do_remote (t:Term) (pTo:Plc) (e:Evidence) (sc : Session_Config)
   let new_att_sesplit_evt := (mkAtt_Sesplit_evt pTo plc_map pk_map) in
   match (map_get plc_map pTo) with 
   | Some uuid => 
-      let remote_req := (mkPRReq new_att_sesplit_evt t my_plc (get_bits e)) in
+      let remote_req := (mkPRReq new_att_sesplit_evt my_plc e t) in
       let js_req := to_JSON remote_req in
       let resp_res := make_JSON_Network_Request uuid js_req in
       match resp_res with
@@ -237,18 +335,22 @@ Definition do_remote (t:Term) (pTo:Plc) (e:Evidence) (sc : Session_Config)
   | None => errC (Unavailable)
   end.
 
-Definition doRemote_session' (t:Term) (pTo:Plc) (e:Evidence) : CVM Evidence := 
+Definition doRemote_session' (pTo:Plc) (e:Evidence) (t:Term) : CVM Evidence := 
   check_cvm_policy t pTo (get_et e) ;;
   sc <- get_config ;;
-  match (do_remote t pTo e sc) with 
-  | resultC ev => err_ret (evc ev (eval t pTo (get_et e)))  
+  match (do_remote sc pTo e t) with 
+  | resultC ev => 
+    match (eval (session_context sc) pTo (get_et e) t) with
+    | resultC e' => err_ret (evc ev e')
+    | errC e => err_failm (dispatch_error (Runtime e))
+    end
   | errC e => err_failm (dispatch_error e)
   end.
 
 Definition remote_session (t:Term) (p:Plc) (q:Plc) (e:Evidence) : CVM Evidence :=
   tag_REQ t p q e ;;
-  e' <- doRemote_session' t q e ;;
-  add_trace (cvm_events t q (get_et e)) ;;
+  e' <- doRemote_session' q e t ;;
+  add_trace (cvm_events q (get_et e) t) ;;
   inc_remote_event_ids t ;;
   err_ret e'.
 
@@ -258,25 +360,23 @@ Definition doRemote (t:Term) (q:Plc) (e:Evidence) : CVM Evidence :=
   tag_RPY p q e' ;;
   err_ret e'.
 
-Definition join_seq (e1:Evidence) (e2:Evidence): CVM unit :=
-  p <- get_pl ;;
-  n <- inc_id ;;
-  put_ev (ss_cons e1 e2) ;;
-  add_trace [join n p].
-
 (* Primitive monadic parallel CVM thread primitives 
    (some rely on Admitted IO Stubs). *)
 
-Definition start_par_thread (loc:Loc) (t:Core_Term) (e:Evidence) : CVM unit :=
+Definition start_par_thread (t: Term) (e:Evidence) : CVM nat :=
   p <- get_pl ;;
-  do_start_par_thread loc t (get_bits e) ;;
-  add_trace [cvm_thread_start loc p t (get_et e)].
+  i <- inc_id ;;
+  (* The loc always = the event id for the thread_start event *)
+  do_start_par_thread i t (get_bits e) ;;
+  add_trace [cvm_thread_start i i p t (get_et e)] ;;
+  err_ret i.
 
-Definition wait_par_thread (loc:Loc) (t:Core_Term) (e:Evidence) : CVM Evidence :=
+Definition wait_par_thread (loc:Loc) (t: Term) (e:Evidence) : CVM Evidence :=
   p <- get_pl ;;
   e' <- do_wait_par_thread loc t p e ;;
-  add_trace [cvm_thread_end loc] ;;
   inc_par_event_ids t ;;
+  i <- inc_id ;;
+  add_trace [cvm_thread_end i loc] ;;
   err_ret e'.
    
 Ltac cvm_monad_unfold :=
@@ -287,7 +387,7 @@ Ltac cvm_monad_unfold :=
   doRemote_session',
   check_cvm_policy,
   invoke_ASP,
-  fwd_asp,
+  bundle_asp,
   extd_bundle,
   comp_bundle,
   encr_bundle,
@@ -300,7 +400,6 @@ Ltac cvm_monad_unfold :=
   get_pl,
   get_config,
   add_trace,
-  modify_evm,
   add_trace in * ;
   repeat err_monad_unfold;
   simpl in * .
