src/Evidence_Bundlers.v
@@ -6,7 +6,7 @@
     Extracted code could be simplified to only the raw EvidenceT operation. *)
 Require Import List String.
 
-Require Import ConcreteEvidenceT ResultT ErrorStringConstants EqClass.
+Require Import Term_Defs ResultT ErrorStringConstants EqClass.
 
 Import ListNotations.
 
@@ -17,7 +17,7 @@ Definition extd_bundle (sig: RawEv) (e:Evidence) (p:Plc) (n : nat) (ps:ASP_PARAM
   match e with
   | evc bits et => 
       if (eqb (List.length sig) n)
-      then resultC (evc (sig ++ bits) (asp_evt p (EXTD n) ps et))
+      then resultC (evc (sig ++ bits) (asp_evt p ps et))
       else errC errStr_raw_EvidenceT_too_long
   end.
 
@@ -28,7 +28,7 @@ Definition comp_bundle (hsh: RawEv) (e:Evidence) (p:Plc) (ps:ASP_PARAMS): Result
   | evc _ et => 
     match hsh with
     | [] => errC errStr_empty_raw_ev
-    | [h] => resultC (evc [h] (asp_evt p COMP ps et))
+    | [h] => resultC (evc [h] (asp_evt p ps et))
     | _ => errC errStr_raw_EvidenceT_too_long
     end
   end.
@@ -41,7 +41,7 @@ Definition encr_bundle (enc: RawEv) (e:Evidence) (p:Plc) (ps:ASP_PARAMS): Result
   | evc _ et => 
     match enc with
     | [] => errC errStr_empty_raw_ev
-    | [h] => resultC (evc [h] (asp_evt p ENCR ps et))
+    | [h] => resultC (evc [h] (asp_evt p ps et))
     | _ => errC errStr_raw_EvidenceT_too_long
     end
   end.
