src/Manifest.v
@@ -60,12 +60,11 @@ Definition PolicyT := list (Plc * ASP_ID).
    *)
   Record Manifest := {
     asps              : manifest_set ASP_ID; 
-    ASP_Compat_Map    : ASP_Compat_MapT;
     ASP_Mapping       : MapC ASP_ID FS_Location;
     man_policy        : PolicyT  ;
     (* TO DO: Add privacy and selection policies to manifest? *)
   }.
 
   Definition empty_Manifest : Manifest :=
-    Build_Manifest nil nil nil nil.
+    Build_Manifest nil nil nil.
 
