src/Manifest_Generator_Facts.v
@@ -1,6 +1,5 @@
 (* Core properties about the Manifest Generator output.
-    Also included:  manifest and environment subset definitions and associated properties. 
-    TODO: consider renaming some of these lemmas (e.g. fafafa, afafafa, ...) *)
+    Also included:  manifest and environment subset definitions and associated properties. *)
 
 Require Import Maps Manifest EqClass Manifest_Generator Manifest_Union.
 
@@ -230,19 +229,31 @@ Proof.
   rewrite String.eqb_eq in *; congruence.
 Qed.
 
-Lemma manifest_generator_cumul : forall t p e1 e2,
+Lemma appr_manifest_update_cumul : forall G et m m',
+  appr_manifest_update G et m = resultC m' ->
+  manifest_subset m m'.
+Proof.
+  induction et; simpl in *; intuition; ff;
+  unfold aspid_manifest_update; 
+  unfold manifest_subset; intuition; 
+  simpl in *; ff; try eapply in_set_add; eauto;
+  ffa using result_monad_unfold.
+Qed.
+
+Lemma manifest_generator_cumul : forall G t et p e1 e2 e',
     Environment_subset e1 e2 ->
-    Environment_subset e1 (manifest_generator' p t e2).
+    manifest_generator' G p et t e2 = resultC e' ->
+    Environment_subset e1 e'.
 Proof.
   intros.
   generalizeEverythingElse t.
-  induction t; intros; try (ff; eauto; fail).
+  induction t; intros; try (ffa using result_monad_unfold; eauto; fail).
   - (* asp case *)
     ff; eauto;
     unfold Environment_subset in *;
     intuition.
-    unfold manifest_update_env, asp_manifest_update, 
-      aspid_manifest_update; try congruence.
+    unfold manifest_update_env_res, asp_manifest_update, 
+      aspid_manifest_update in *; try congruence;
     ff; subst; find_apply_hyp_hyp; break_exists;
     intuition; destEq p0 p;
     repeat find_rewrite; repeat find_injection;
@@ -257,17 +268,19 @@ Proof.
     eexists; intuition; eauto;
     unfold manifest_subset in *; intuition; simpl in *;
     find_apply_hyp_hyp; eauto;
-    eapply in_set_add; eauto.
-  - simpl in *; ff.
+    try (eapply in_set_add; eauto);
+    find_apply_lem_hyp appr_manifest_update_cumul; eauto.
+  - simpl in *; ffa;
     eapply IHt;
-    eapply env_subset_cons_none; eauto.
+    [ eapply env_subset_cons_none; eauto | eauto ].
 Qed.
 
-Lemma manifest_generator_cumul' : forall t p e,
-  Environment_subset e (manifest_generator' p t e).
+Lemma manifest_generator_cumul' : forall G t et p e e',
+  manifest_generator' G p et t e = resultC e' ->
+  Environment_subset e e'.
 Proof.
   intros.
-  apply manifest_generator_cumul.
+  eapply manifest_generator_cumul; eauto;
   apply env_subset_refl.
 Qed.
 
@@ -306,118 +319,15 @@ Proof.
   rewrite String.eqb_eq in *; subst; eauto.
 Qed.
 
-Lemma fafafa : forall t p e1 e2,
-    Environment_subset e1 e2 ->
-    Environment_subset (manifest_generator' p t e1)
-                       (manifest_generator' p t e2).
-Proof.
-  intros.
-  generalizeEverythingElse t.
-  induction t; intros; eauto.
-  - (* asp case *)
-    destruct a; ff;
-    unfold manifest_update_env, asp_manifest_update,
-      aspid_manifest_update, Environment_subset, 
-      empty_Manifest in *; ff;
-    simpl in *; intuition; eauto;
-
-
-    try match goal with 
-    | H1 : map_get e1 ?p1 = _,
-      H2 : map_get (map_set e1 ?p1 _) ?p2 = Some ?m2 |- _ =>
-        destruct (eqb p1 p2) eqn:E;
-
-        [
-          rewrite eqb_eq in *; subst;
-          (* try (destruct (H _ _ H1); intuition; eauto). *)
-          unfold manifest_subset in *; simpl in *;
-          rewrite mapC_get_works in *;
-          repeat find_rewrite; repeat find_injection; simpl in *; eauto;
-          eexists; simpl in *; intuition; simpl in *; eauto; try congruence;
-          try find_apply_hyp_hyp;
-          destruct_conjs; ff;
-          try find_rewrite; repeat find_injection; ff;
-
-
-
-          try match goal with 
-          | H1 : In_set _ (manset_add _ _) |- _ => 
-            apply manadd_In_set in H1;
-          door; subst;
-          try (find_apply_hyp_hyp);
-            try (eapply manadd_In_add);
-            try (eapply in_set_add);
-          eauto
-          end;
-
-          try (apply manadd_In_add); try (subst; apply manadd_In_add)
-      
-
-          | 
-          assert (p1 <> p2) by (intros HC; rewrite <- eqb_eq in HC; congruence);
-          assert (HM : map_get e1 p2 = Some m2) by (eapply mapC_get_distinct_keys_from_set; eauto);
-          destruct (H _ _ HM); intuition; eauto;
-          erewrite mapC_get_distinct_keys; eauto
-
-
-
-        ]
-      end. 
-  - simpl in *; ff; eapply IHt; eauto. 
-    * unfold Environment_subset in *; intuition.
-      eapply H in Heqo; break_exists; find_rewrite; 
-      intuition; congruence.
-    * eapply env_subset_l_cons; eauto.
-    * eapply env_subset_both_cons; eauto. 
-Qed.
-
-Lemma map_get_mangen : forall t e p p' v,
+Lemma map_get_mangen : forall G t et e e' p p' v,
   map_get e p = Some v ->
+  manifest_generator' G p' et t e = resultC e' ->
   exists v',
-  map_get (manifest_generator' p' t e) p = Some v'.
+  map_get e' p = Some v'.
 Proof.
-  intros.
-  assert (Environment_subset e (manifest_generator' p' t e)).
-  {
-    apply manifest_generator_cumul.
-    apply env_subset_refl.
-  }
-
-  unfold Environment_subset in H0.
-  specialize H0 with (m1:=v) (p:=p).
-  apply H0 in H.
-  destruct_conjs.
-  eexists.
-  apply H1.
-Qed.
-
-
-Lemma afafa : forall e p t p0 m m',
-  map_get (manifest_generator' p t e) p0 = Some m -> 
-  e = [(p0, m')] ->
-  manifest_subset m' m.
-Proof.
-  intros.
-  subst.
-
-  assert (
-    Environment_subset 
-      [(p0, m')] 
-      (manifest_generator' p t [(p0, m')])
-  ).
-  {
-    apply manifest_generator_cumul.
-    apply env_subset_refl.
-  }
-
-  unfold Environment_subset in H0.
-  specialize H0 with (m1:=m') (p:=p0).
-  assert (map_get [(p0, m')] p0 = Some m').
-  {
-    simpl in *; rewrite String.eqb_refl; eauto.
-  }
-  apply H0 in H1.
-  destruct_conjs.
-  rewrite H2 in *.
-  ff.
+  intros;
+  find_apply_lem_hyp manifest_generator_cumul';
+  unfold Environment_subset in *;
+  find_apply_hyp_hyp;
+  break_exists; intuition; ff.
 Qed.
