src/Manifest_Generator_Union.v
@@ -13,74 +13,7 @@ Require Import Manifest_Union Manifest_Generator.
 Require Import List.
 Import ListNotations.
 
-Definition manifest_generator_plcTerm_list (ls:list (Term*Plc)) : list EnvironmentM := 
-    List.map (fun '(t,p) => manifest_generator t p) ls.
-
-Definition env_list_union (ls:list EnvironmentM) : EnvironmentM := 
-    fold_right environment_union e_empty ls.
-
-Definition mangen_plcTerm_list_union (ls:list (Term*Plc)) : EnvironmentM := 
-    env_list_union (manifest_generator_plcTerm_list ls).
-
-Definition manifest_generator_plcEvidenceT_list (comp_map : ASP_Compat_MapT) 
-    (ls:list (EvidenceT*Plc)) : ResultT (list EnvironmentM) string := 
-  result_map (fun '(et,p) => manifest_generator_app comp_map et p) ls.
-
-Definition mangen_plcEvidenceT_list_union (comp_map : ASP_Compat_MapT) 
-    (ls:list (EvidenceT*Plc)) : ResultT EnvironmentM string := 
-  match (manifest_generator_plcEvidenceT_list comp_map ls) with
-  | resultC ls' => resultC (env_list_union ls')
-  | errC e => errC e
-  end.
-
-Definition EvidenceT_Plc_list := list (EvidenceT*Plc).
 Open Scope string_scope.
-
-Definition EvidenceT_Plc_list_to_JSON `{Jsonifiable EvidenceT} (ls: EvidenceT_Plc_list) : JSON := 
-  JSON_Object [
-    ("EvidenceT_Plc_list",
-      (JSON_Array 
-        (List.map 
-          (fun '(et,p) => 
-            JSON_Array [
-              to_JSON et;
-              JSON_String (to_string p)
-            ]
-          ) ls)
-      )
-    )].
-
-Definition EvidenceT_Plc_list_from_JSON `{Jsonifiable EvidenceT, Jsonifiable ASP_Compat_MapT} (js : JSON) 
-    : ResultT EvidenceT_Plc_list string :=
-  match (JSON_get_Array "EvidenceT_Plc_list" js) with
-  | resultC jsArr =>
-    let res := result_map (fun js => 
-      match js with
-      | JSON_Array [jsEt; JSON_String jsP] =>
-        match (from_JSON jsEt), (from_string jsP) with
-        | resultC et,resultC p => resultC (et, p)
-        | _, _ => errC "Error in parsing EvidenceT_Plc_list"
-        end
-      | _ => errC "Not a pair"
-      end
-    ) jsArr in
-    match res with
-    | resultC res => resultC res
-    | errC e => errC e
-    end
-  | errC e => errC e 
-  end.
-
-Global Instance Jsonifiable_EvidenceT_Plc_list `{Jsonifiable EvidenceT} : Jsonifiable EvidenceT_Plc_list.
-eapply Build_Jsonifiable with 
-  (to_JSON := EvidenceT_Plc_list_to_JSON)
-  (from_JSON := EvidenceT_Plc_list_from_JSON).
-unfold EvidenceT_Plc_list_to_JSON, EvidenceT_Plc_list_from_JSON;
-induction a; simpl in *; intuition;
-repeat (try break_match; simpl in *; subst; try congruence);
-repeat rewrite canonical_jsonification in *; try congruence;
-repeat find_injection; eauto.
-Defined.
 
 Definition Term_Plc_list := list (Term*Plc).
 
@@ -129,25 +62,8 @@ repeat rewrite canonical_jsonification in *; try congruence;
 repeat find_injection; eauto.
 Defined.
 
-Definition end_to_end_mangen (comp_map : ASP_Compat_MapT) 
-    (ls: EvidenceT_Plc_list) (ts: Term_Plc_list) 
+Definition end_to_end_mangen (G : GlobalContext) (ts: Term_Plc_list) 
     : ResultT EnvironmentM string := 
-  let app_env := mangen_plcEvidenceT_list_union comp_map ls in
-  let att_env := mangen_plcTerm_list_union ts in 
-  match app_env with
-  | resultC app_env => resultC (environment_union app_env 
-      (Maps.map_map (fun m => add_compat_map_manifest m comp_map) att_env))
-  | errC e => errC e
-  end.
+  result_fold (fun '(t,p) => fun env =>
+    manifest_generator G p t) e_empty ts.
 
-Definition manset_union_list{A : Type} `{HA : EqClass A} 
-  (lss: manifest_set (manifest_set A)) : manifest_set A := 
-    fold_right manset_union [] lss.
-
-Definition end_to_end_mangen_final (comp_map : ASP_Compat_MapT) 
-    (ls: EvidenceT_Plc_list) (ts: Term_Plc_list) 
-    : ResultT (list Manifest) string :=
-  match (end_to_end_mangen comp_map ls ts) with
-  | resultC env => resultC (environment_to_manifest_list env)
-  | errC e => errC e
-  end.
