src/Manifest_JSON.v
@@ -4,13 +4,11 @@ Import ListNotations ResultNotation.
 
 
 Definition Manifest_to_JSON (m : Manifest) : JSON :=
-  let '(Build_Manifest asps asp_compat_map asp_fs_map policy) := m 
+  let '(Build_Manifest asps asp_fs_map policy) := m 
   in
     JSON_Object [
       (MAN_ASPS, 
         (JSON_Array (manifest_set_to_list_JSON asps)));
-      (MAN_ASP_COMPAT_MAP, 
-        (to_JSON asp_compat_map));
       (MAN_ASP_FS_MAP, 
         (to_JSON asp_fs_map));
       (MAN_POLICY, 
@@ -19,15 +17,13 @@ Definition Manifest_to_JSON (m : Manifest) : JSON :=
 
 Definition JSON_to_Manifest (js : JSON) : ResultT Manifest string :=
   temp_ASPS <- JSON_get_Array MAN_ASPS js;;
-  temp_ASP_COMPAT_MAP <- JSON_get_Object MAN_ASP_COMPAT_MAP js;;
   temp_ASP_FS_MAP <- JSON_get_Object MAN_ASP_FS_MAP js;;
   temp_POLICY <- JSON_get_Array MAN_POLICY js;;
 
   ASPS <- list_JSON_to_manifest_set temp_ASPS;;
-  ASP_COMPAT_MAP <- from_JSON temp_ASP_COMPAT_MAP;;
   ASP_FS_MAP <- from_JSON temp_ASP_FS_MAP;;
   POLICY <- list_JSON_to_manifest_set_pairs temp_POLICY;;
-  resultC (Build_Manifest ASPS ASP_COMPAT_MAP ASP_FS_MAP POLICY).
+  resultC (Build_Manifest ASPS ASP_FS_MAP POLICY).
 
 Global Instance Jsonifiable_Manifest `{Jsonifiable (MapC ASP_ID FS_Location), Jsonifiable (ASP_Compat_MapT)}: Jsonifiable Manifest. 
 eapply Build_Jsonifiable with 
@@ -35,8 +31,6 @@ eapply Build_Jsonifiable with
   JSON_Object [
     (MAN_ASPS, 
       (JSON_Array (manifest_set_to_list_JSON (asps m))));
-    (MAN_ASP_COMPAT_MAP, 
-      (to_JSON (ASP_Compat_Map m)));
     (MAN_ASP_FS_MAP, 
       (to_JSON (ASP_Mapping m)));
     (MAN_POLICY, 
@@ -44,15 +38,13 @@ eapply Build_Jsonifiable with
   ]))
 (from_JSON := (fun js =>
     temp_ASPS <- JSON_get_Array MAN_ASPS js;;
-  temp_ASP_COMPAT_MAP <- JSON_get_Object MAN_ASP_COMPAT_MAP js;;
   temp_ASP_FS_MAP <- JSON_get_Object MAN_ASP_FS_MAP js;;
   temp_POLICY <- JSON_get_Array MAN_POLICY js;;
 
   ASPS <- list_JSON_to_manifest_set temp_ASPS;;
-  ASP_COMPAT_MAP <- from_JSON temp_ASP_COMPAT_MAP;;
   ASP_FS_MAP <- from_JSON temp_ASP_FS_MAP;;
   POLICY <- list_JSON_to_manifest_set_pairs temp_POLICY;;
-  resultC (Build_Manifest ASPS ASP_COMPAT_MAP ASP_FS_MAP POLICY))).
+  resultC (Build_Manifest ASPS ASP_FS_MAP POLICY))).
 simpl_json; rewrite canonical_list_injson_to_manset;
 rewrite canonical_list_injson_to_manset_pairs; solve_json.
 Defined.
